Simple, "working" separation logic prover. - Not all cases are handled, not everything is verified.

src/SepExpr.v
@@ -1,11 +1,10 @@
 Require Import List.
 Require Import Expr.
 Require Import Heaps PropX.
+Require Import PropXTac.
 Require Import PMap.
 
 Set Implicit Arguments.
-
-Require Import PropXTac.
 
 Ltac goPropX := 
   repeat match goal with
@@ -27,9 +26,11 @@ Module SepExpr (B : Heap).
     Variable stateType : tvar types.
     Variable stateMem : tvarD stateType -> B.mem.
 
+    Definition hprop : Type := HT.smem -> PropX (tvarD pcType) (tvarD stateType).
+
     Record ssignature := {
       SDomain : list (tvar types) ;
-      SDenotation : functionTypeD (map (@tvarD types) SDomain) (HT.smem -> PropX (tvarD pcType) (tvarD stateType))
+      SDenotation : functionTypeD (map (@tvarD types) SDomain) hprop
     }.
     Variable sfuncs : list ssignature.
 
@@ -43,6 +44,7 @@ Module SepExpr (B : Heap).
     | Cptr : forall vars, expr funcs vars pcType -> sexpr (stateType :: vars) -> sexpr vars
     | Func : forall vars (f : fin sfuncs), 
       hlist (expr funcs vars) (SDomain (get sfuncs f)) -> sexpr vars
+      (* this Const can not mention the higher-order variables *)
     | Const : forall vars, fin consts -> sexpr vars
     (** If PtsTo is derived: we can handle different sizes easily, 
      ** If PtsTo is built-in: we can derive <> facts easily (also precision)
@@ -53,134 +55,148 @@ Module SepExpr (B : Heap).
      **)
 
 
-    Fixpoint sexprD (vars : variables types) (s : sexpr vars)
-      : hlist (@tvarD types)  vars -> HT.smem -> PropX (tvarD pcType) (tvarD stateType) :=
-      match s in sexpr vars return hlist (@tvarD types) vars -> HT.smem -> PropX (tvarD pcType) (tvarD stateType) with
-        | Inj _ p => fun g _ => PropX.Inj (exprD g p)
-        | Exists _ t b => fun g m => PropX.Exists (fun x : tvarD t => @sexprD _ b (HCons x g) m)
-        | Func _ f b => fun g =>
-          applyD (exprD g) b _ (SDenotation (get sfuncs f))
-        | Const _ p => fun _ _ =>
-          get consts p
+    Fixpoint sexprD vars (s : sexpr vars)
+      : hlist (@tvarD types) vars -> HT.smem -> PropX (tvarD pcType) (tvarD stateType) :=
+      match s in sexpr vs
+        return hlist (@tvarD types) vs ->  HT.smem -> PropX (tvarD pcType) (tvarD stateType) 
+        with
+        | Emp v => fun g m => 
+          PropX.Inj (HT.semp m)
+        | Inj v p => fun g m => 
+          PropX.And (PropX.Inj (exprD g p)) (PropX.Inj (HT.semp m))
         | Star _ l r => fun g m => 
           PropX.Exists (fun ml : HT.smem => PropX.Exists (fun mr : HT.smem => 
             PropX.And (PropX.Inj (HT.split m ml mr)) (And (sexprD l g ml) (sexprD r g mr))))
-        | Emp _ => fun _ m => 
-          PropX.Inj (HT.semp m)
+        | Exists _ t b => fun g m => PropX.Exists (fun x : tvarD t => @sexprD _ b (HCons x g) m)
         | Cptr _ p t => fun g m =>
-          PropX.Cptr (exprD g p) 
-          (fun x : tvarD stateType => PropX.Exists (fun m => 
-            PropX.And (PropX.Inj (HT.satisfies m (stateMem x))) (sexprD t (HCons x g) m)))
+          PropX.And 
+            (PropX.Inj (HT.semp m))
+            (PropX.Cptr (exprD g p) 
+              (fun x : tvarD stateType => PropX.Exists (fun m => 
+                PropX.And (PropX.Inj (HT.satisfies m (stateMem x))) (sexprD t (HCons x g) m))))
+        | Func _ f b => fun g =>
+          applyD (exprD g) b _ (SDenotation (get sfuncs f))
+        | Const _ p => fun _ m =>
+          PropX.And (PropX.Inj (HT.semp m)) (get consts p)
       end.
 
     Section Cmp.
-      Definition sexprCmp vars (a : sexpr vars) : forall b, dcomp a b.
-        refine ((fix sexprCmp vars (a : sexpr vars) {struct a} : forall b, dcomp a b :=
-          match a in sexpr vars return forall b : sexpr vars, dcomp a b with
+      Definition sexprCmp vars (a : sexpr vars) : forall b, option (dcomp a b).
+        refine ((fix sexprCmp vars (a : sexpr vars) {struct a} : forall b, option (dcomp a b) :=
+          match a in sexpr vars return forall b : sexpr vars, option (dcomp a b) with
             | Emp _ => fun b =>
               match b with
-                | Emp _ => Env.Eq _
-                | _ => Env.Lt _ _
+                | Emp _ => Some (Env.Eq _)
+                | _ => Some (Env.Lt _ _)
               end
             | Inj v l => fun b =>
-              match b in sexpr v' return forall l : expr funcs v' None, dcomp (Inj l) b with
+              match b in sexpr v' return forall l : expr funcs v' None, option (dcomp (Inj l) b) with
                 | Inj _ r => fun l => match exprEq l r with
-                                        | Some _ => Env.Eq _
-                                        | None => Env.Lt _ _ (** TODO: This is wrong! **)
+                                        | Some _ => Some (Env.Eq _)
+                                        | None => None
                                       end
-                | Emp _ => fun _ => Gt _ _
-                | _ => fun _ => Lt _ _ 
+                | Emp _ => fun _ => Some (Gt _ _)
+                | _ => fun _ => Some (Lt _ _)
               end l
             | Star v ll lr => fun b =>
               match b in sexpr v' 
-                return forall (Heq : v' = v), (forall (x y : sexpr v'), dcomp (Star ll lr) (match Heq in _ = t 
-                                                                                              return sexpr t
-                                                                                              with
-                                                                                              | refl_equal => Star x y
-                                                                                            end))
-                -> dcomp (Star ll lr) (match Heq in _ = t return sexpr t with
-                                         | refl_equal => b
-                                       end)
+                return forall (Heq : v' = v), (forall (x y : sexpr v'), option (dcomp (Star ll lr) (match Heq in _ = t 
+                                                                                                      return sexpr t
+                                                                                                      with
+                                                                                                      | refl_equal => Star x y
+                                                                                                    end)))
+                -> option (dcomp (Star ll lr) (match Heq in _ = t return sexpr t with
+                                                 | refl_equal => b
+                                               end))
                 with
                 | Star _ rl rr => fun _ cc => cc rl rr
-                | Emp _ | Inj _ _ => fun _ _ => Env.Gt _ _ 
-                | _ => fun _ _ => Env.Lt _ _ 
+                | Emp _ | Inj _ _ => fun _ _ => Some (Env.Gt _ _)
+                | _ => fun _ _ => Some (Env.Lt _ _)
               end (refl_equal _)
               (fun (x y : sexpr v) =>
                 match sexprCmp _ ll x with
-                  | Env.Lt => Env.Lt _ _
-                  | Env.Gt => Env.Gt _ _
-                  | Env.Eq _ => 
+                  | Some Env.Lt => Some (Env.Lt _ _)
+                  | Some Env.Gt => Some (Env.Gt _ _)
+                  | Some (Env.Eq _) => 
                     match sexprCmp _ lr y with
-                      | Env.Lt => Env.Lt _ _
-                      | Env.Gt => Env.Gt _ _
-                      | Env.Eq _ => Env.Eq _
+                      | Some Env.Lt => Some (Env.Lt _ _)
+                      | Some Env.Gt => Some (Env.Gt _ _)
+                      | Some (Env.Eq _) => Some (Env.Eq _)
+                      | None => None
                     end
+                  | None => 
+                    match sexprCmp _ lr y with
+                      | Some Env.Lt => Some (Env.Lt _ _)
+                      | Some Env.Gt => Some (Env.Gt _ _)
+                      | _ => None
+                    end                    
                 end)
             | Exists v t body => fun b =>
               match b in sexpr v' 
                 return forall (Heq : v' = v),
-                  (forall t' (x : sexpr (t' :: v')), t' = t -> dcomp (Exists body) (match Heq in _ = t 
-                                                                                      return sexpr t 
-                                                                                      with
-                                                                                      | refl_equal => Exists x
-                                                                                    end)) ->
-                  dcomp (Exists body) (match Heq in _ = t return sexpr t with
-                                         | refl_equal => b
-                                       end)
+                  (forall t' (x : sexpr (t' :: v')), t' = t -> option (dcomp (Exists body) (match Heq in _ = t 
+                                                                                              return sexpr t 
+                                                                                              with
+                                                                                              | refl_equal => Exists x
+                                                                                            end))) ->
+                  option (dcomp (Exists body) (match Heq in _ = t return sexpr t with
+                                                 | refl_equal => b
+                                               end))
                 with
                 | Exists v' t' b' => fun Heq cc =>
                   match tvar_dec t' t with
                     | left pf => cc _ _ _
-                    | right _ => Env.Lt _ _ (** TODO: wrong **)
+                    | right _ => None
                   end
-                | Emp _ | Inj _ _ | Star _ _ _ => fun _ _ => Env.Gt _ _
-                | _ => fun _ _ => Env.Lt _ _ 
+                | Emp _ | Inj _ _ | Star _ _ _ => fun _ _ => Some (Env.Gt _ _)
+                | _ => fun _ _ => Some (Env.Lt _ _)
               end (refl_equal _)
               (fun t x eqq => 
                 match sexprCmp _ body match eqq in _ = t' return sexpr (t' :: v) with
                                         | refl_equal => x
                                       end
                   with
-                  | Env.Lt => Env.Lt _ _
-                  | Env.Gt => Env.Gt _ _
-                  | Env.Eq _ => Env.Eq _
+                  | Some Env.Lt => Some (Env.Lt _ _)
+                  | Some Env.Gt => Some (Env.Gt _ _)
+                  | Some (Env.Eq _) => Some (Env.Eq _)
+                  | None => None
                 end)
             | Cptr v lp ls => fun b =>
               match b in sexpr v' 
                 return forall (Heq : v' = v), 
-                  (forall (p : expr funcs v' pcType) (s : sexpr (stateType :: v')), dcomp (Cptr lp ls) (match Heq in _ = t
-                                                                                                          return sexpr t
-                                                                                                          with 
-                                                                                                          | refl_equal => Cptr p s
-                                                                                                        end)) ->
-                  dcomp (Cptr lp ls) (match Heq in _ = t return sexpr t with
-                                        | refl_equal => b
-                                      end)
+                  (forall (p : expr funcs v' pcType) (s : sexpr (stateType :: v')), 
+                    option (dcomp (Cptr lp ls) (match Heq in _ = t
+                                                  return sexpr t
+                                                  with 
+                                                  | refl_equal => Cptr p s
+                                                end))) ->
+                  option (dcomp (Cptr lp ls) (match Heq in _ = t return sexpr t with
+                                                | refl_equal => b
+                                              end))
                 with
                 | Cptr _ rp rs => fun _ cc => cc rp rs
-                | Emp _ | Inj _ _ | Star _ _ _ | Exists _ _ _ => fun _ _ => Env.Gt _ _
-                | _ => fun _ _ => Env.Lt _ _
+                | Emp _ | Inj _ _ | Star _ _ _ | Exists _ _ _ => fun _ _ => Some (Env.Gt _ _)
+                | _ => fun _ _ => Some (Env.Lt _ _)
               end (refl_equal _)
               (fun x y =>
                 match exprEq lp x with
                   | Some _ => match sexprCmp _ ls y with
-                                | Env.Eq _ => Env.Eq _
-                                | Env.Gt => Env.Gt _ _
-                                | Env.Lt => Env.Lt _ _
-                              end
-                    
-                  | _ => Env.Lt _ _ (** TODO: Wrong **)
+                                | Some (Env.Eq _) => Some (Env.Eq _)
+                                | Some Env.Gt => Some (Env.Gt _ _)
+                                | Some Env.Lt => Some (Env.Lt _ _)
+                                | None => None
+                              end                    
+                  | _ => None
                 end)
             | Func v f args => fun b =>
               match b in sexpr v'
                 return forall (Heq : v' = v), 
                   (forall args', option (args = args')) ->
-                  dcomp (Func f args) (match Heq in _ = t 
-                                          return sexpr t
-                                          with
-                                          | refl_equal => b
-                                        end)
+                  option (dcomp (Func f args) (match Heq in _ = t 
+                                                 return sexpr t
+                                                 with
+                                                 | refl_equal => b
+                                               end))
                 with
                 | Func v' f' args' => fun Heq cc => 
                   match finCmp f f' with
@@ -193,23 +209,23 @@ Module SepExpr (B : Heap).
                                                             end
                                           end
                                    with
-                                   | Some _ => Env.Eq  _
-                                   | None => Env.Lt _ _ (** TODO : Wrong **)
+                                   | Some _ => Some (Env.Eq _)
+                                   | None => None
                                  end                                     
-                    | Env.Lt => Env.Lt _ _ 
-                    | Env.Gt => Env.Gt _ _
+                    | Env.Lt => Some (Env.Lt _ _)
+                    | Env.Gt => Some (Env.Gt _ _)
                   end
-                | Emp _ | Inj _ _ | Star _ _ _ | Exists _ _ _ | Cptr _ _ _ => fun _ _ => Env.Gt _ _
-                | _ => fun _ _ => Env.Lt _ _
+                | Emp _ | Inj _ _ | Star _ _ _ | Exists _ _ _ | Cptr _ _ _ => fun _ _ => Some (Env.Gt _ _)
+                | _ => fun _ _ => Some (Env.Lt _ _)
               end (refl_equal _) (hlistEq (@exprEq _ _ _) args)
             | Const _ x => fun b => 
               match b with
                 | Const _ y => match finCmp x y with
-                                 | Env.Eq _ => Env.Eq _ 
-                                 | Env.Lt => Env.Lt _ _
-                                 | Env.Gt => Env.Gt _ _
+                                 | Env.Eq _ => Some (Env.Eq _)
+                                 | Env.Lt => Some (Env.Lt _ _)
+                                 | Env.Gt => Some (Env.Gt _ _)
                                end
-                | _ => Env.Gt _ _ 
+                | _ => Some (Env.Gt _ _)
               end
           end) vars a);
         clear sexprCmp; try abstract (subst; reflexivity).
@@ -227,6 +243,8 @@ Module SepExpr (B : Heap).
 
       Definition himp (gl gr : sexpr vars) : Prop :=
         forall m, valid cs nil (sexprD gl G m) -> valid cs nil (sexprD gr G m).
+      Definition heq (gl gr : sexpr vars) : Prop :=
+        forall m, valid cs nil (sexprD gl G m) <-> valid cs nil (sexprD gr G m).
 
       Require Import RelationClasses.
 
@@ -264,7 +282,8 @@ Module SepExpr (B : Heap).
       Theorem star_assoc_p : forall P Q R S,
         himp (Star P (Star Q R)) S -> himp (Star (Star P Q) R) S.
       Proof.
-        doIt. apply HT.split_comm. apply HT.split_comm in H. eapply HT.split_assoc; try eassumption. apply HT.split_comm. eassumption. eapply HT.disjoint_split_join.
+        doIt. apply HT.split_comm. apply HT.split_comm in H. eapply HT.split_assoc; try eassumption. 
+        apply HT.split_comm. eassumption. eapply HT.disjoint_split_join.
         apply HT.disjoint_comm. eapply HT.split_split_disjoint; eauto.
         apply HT.split_comm in H0; eassumption.
       Qed.
@@ -286,6 +305,18 @@ Module SepExpr (B : Heap).
         doIt. eassumption. cut (valid cs nil (sexprD R G x0)). intros. doIt. apply H.
         doIt.
       Qed.
+
+      Theorem star_frame : forall P Q R S, himp P Q -> himp R S -> himp (Star P R) (Star Q S).
+      Proof.
+        unfold himp; simpl; intros;
+          repeat match goal with
+                   | [ H : _ -> _ |- _ ] => apply H; clear H
+                   | [ H : ?X -> _ , H' : ?X |- _ ] => apply H in H'; clear H
+                 end; goPropX.
+        apply simplify_bwd in H2. apply simplify_bwd in H3. apply H in H2. apply H0 in H3. doIt.
+        assumption.
+      Qed.
+
 (*
       Lemma valid_smem_eq : forall vars (P : sexpr vars) G E m m',
         valid cs E (sexprD P G m) -> HT.smem_eq m m' -> valid cs E (sexprD P G m').
@@ -318,7 +349,7 @@ Module SepExpr (B : Heap).
       Definition Himp := @himp nil HNil.
 
       Inductive SepResult (cs : codeSpec (tvarD pcType) (tvarD stateType)) (gl gr : sexpr nil) : Type :=
-      | Solved : Himp cs gl gr -> SepResult cs gl gr
+      | Proved : Himp cs gl gr -> SepResult cs gl gr
       | Remaining : forall l r, (Himp cs l r -> Himp cs gl gr) -> SepResult cs gl gr.
 
       Definition SProverT : Type := forall
@@ -339,7 +370,7 @@ Module SepExpr (B : Heap).
   Implicit Arguments Func [ types funcs pcType stateType sfuncs consts vars ].
   Implicit Arguments Const [ types funcs pcType stateType sfuncs consts vars ].
 
-  Implicit Arguments Solved [ types funcs pcType stateType stateMem sfuncs consts cs gl gr ].
+  Implicit Arguments Proved [ types funcs pcType stateType stateMem sfuncs consts cs gl gr ].
   Implicit Arguments Remaining [ types funcs pcType stateType stateMem sfuncs consts cs gl gr ].
 
   Section BabySep.
@@ -354,33 +385,15 @@ Module SepExpr (B : Heap).
     Definition ReflSep : @SProverT types fs pcType stateType stateMem sfuncs consts.
     red. refine (fun _ _ gl gr =>
       match sexprCmp gl gr with
-        | Env.Eq _ => Solved _
+        | Some (Env.Eq _) => Proved _
         | _ => Remaining gl gr _ 
       end); eauto.
     subst. unfold Himp, himp, himp. auto.
     Defined.
 
-    Require Import PMap.
-
-    Parameter map : Type -> Type -> Type.
-
-    Parameter dmap_join : forall {K} {V}, @dmap K V -> dmap K V -> dmap K V.
-    Parameter map_empty : forall K V, map K V.
-    Parameter map_fold : forall {A} {K} {V} (f : A -> K -> V -> A) (a : A) (m : map K V), A.
-    Parameter map_insert : forall {K} {V}, K -> V -> @map K V -> map K V.
-    Parameter map_join : forall {K} {V}, map K V -> @map K V -> map K V.
-    Parameter map_remove : forall {K} {V}, K -> map K V -> option (V * map K V).
-
-    Parameter dmap_join_empty : forall {K} {V} (v : @dmap K V), dmap_join dmap_empty v = v.
-    Parameter map_join_empty : forall {K} {V} (v : map K V), map_join (map_empty _ _) v = v.
-    
-    Parameter dmap_fold_empty : forall A K V f (a : A), dmap_fold f a (@dmap_empty K V) = a.
-    Parameter map_fold_empty : forall A K V f (a : A), map_fold f a (@map_empty K V) = a.
-
-
     Record SHeap vars : Type :=
     { funcs  : @dmap (fin sfuncs) (fun f => list (hlist (expr fs vars) (SDomain (get sfuncs f))))
-    ; cptrs  : map (expr fs vars pcType) (sexpr fs sfuncs consts (stateType :: vars))
+    ; cptrs  : fmap (expr fs vars pcType) (sexpr fs sfuncs consts (stateType :: vars))
     ; pures  : list (expr fs vars None)
     ; cnsts  : list (fin consts)
     ; other  : list (sexpr fs sfuncs consts vars)
@@ -388,15 +401,15 @@ Module SepExpr (B : Heap).
   
     Definition SHeap_empty vars : SHeap vars := 
       {| funcs := dmap_empty
-        ; cptrs := map_empty _ _
-        ; pures := nil
-        ; cnsts := nil
-        ; other := nil
-        |}.
+       ; cptrs := fmap_empty
+       ; pures := nil
+       ; cnsts := nil
+       ; other := nil
+       |}.
 
     Definition denote vars (h : SHeap vars) :  sexpr fs sfuncs consts vars :=
       let a := dmap_fold (fun a x y => fold_left (fun a y => Star (Func x y) a) y a) Emp (funcs h) in
-      let b := map_fold (fun a x y => Star (Cptr x y) a) Emp (cptrs h) in
+      let b := fmap_fold (fun a x y => Star (Cptr x y) a) Emp (cptrs h) in
       let c := fold_right (fun x a => Star (Inj x) a) Emp (pures h) in
       let d := fold_right (fun x a => Star (Const x) a) Emp (cnsts h) in
       let e := fold_right (fun x a => Star x a) Emp (other h) in
@@ -404,12 +417,12 @@ Module SepExpr (B : Heap).
 
     Fixpoint hash_rec T vars (s : sexpr fs sfuncs consts vars) 
       :  (   @dmap (fin sfuncs) (fun f => list (hlist (expr fs vars) (SDomain (get sfuncs f))))
-          -> map (expr fs vars pcType) (sexpr fs sfuncs consts (stateType :: vars))
+          -> fmap (expr fs vars pcType) (sexpr fs sfuncs consts (stateType :: vars))
           -> list (expr fs vars None)
           -> list (fin consts)
           -> list (sexpr fs sfuncs consts vars) -> T)
       -> @dmap (fin sfuncs) (fun f => list (hlist (expr fs vars) (SDomain (get sfuncs f))))
-      -> map (expr fs vars pcType) (sexpr fs sfuncs consts (stateType :: vars))
+      -> fmap (expr fs vars pcType) (sexpr fs sfuncs consts (stateType :: vars))
       -> list (expr fs vars None)
       -> list (fin consts)
       -> list (sexpr fs sfuncs consts vars)
@@ -417,12 +430,12 @@ Module SepExpr (B : Heap).
       match s in @sexpr _ _ _ _ _ _ vs 
         return 
            (   @dmap (fin sfuncs) (fun f => list (hlist (expr fs vs) (SDomain (get sfuncs f))))
-            -> map (expr fs vs pcType) (sexpr fs sfuncs consts (stateType :: vs))
+            -> fmap (expr fs vs pcType) (sexpr fs sfuncs consts (stateType :: vs))
             -> list (expr fs vs None)
             -> list (fin consts)
             -> list (sexpr fs sfuncs consts vs) -> T)
         -> @dmap (fin sfuncs) (fun f => list (hlist (expr fs vs) (SDomain (get sfuncs f))))
-        -> map (expr fs vs pcType) (sexpr fs sfuncs consts (stateType :: vs))
+        -> fmap (expr fs vs pcType) (sexpr fs sfuncs consts (stateType :: vs))
         -> list (expr fs vs None)
         -> list (fin consts)
         -> list (sexpr fs sfuncs consts vs)
@@ -434,14 +447,14 @@ Module SepExpr (B : Heap).
         | Star _ l r => fun cc =>
           hash_rec l (hash_rec r cc)
         | Func _ f args => fun cc fs cps ps cs ot =>
-          match dmap_remove (@finCmp _ _) f fs with
+          match dmap_remove (fun a b => Some (@finCmp _ _ a b)) f fs with
             | None =>
-              cc (dmap_insert (@finCmp _ _) f (args :: nil) fs) cps ps cs ot
+              cc (dmap_insert (fun a b => Some (@finCmp _ _ a b)) f (args :: nil) fs) cps ps cs ot
             | Some (v,fs') =>
-              cc (dmap_insert (@finCmp _ _) f (args :: v) fs') cps ps cs ot
+              cc (dmap_insert (fun a b => Some (@finCmp _ _ a b)) f (args :: v) fs') cps ps cs ot
           end
         | Cptr _ p s => fun cc fs cps ps cs ot =>
-          cc fs (map_insert p s cps) ps cs ot 
+          cc fs (fmap_insert (@exprCmp _ _ _ _ ) p s cps) ps cs ot 
         | x => fun cc fs cps ps cs ot =>
           (** TODO : Other cases are problematic... **)
           cc fs cps ps cs (x :: ot)
@@ -449,24 +462,87 @@ Module SepExpr (B : Heap).
 
     Definition hash_cc T vars (s : sexpr fs sfuncs consts vars)
       (cc : @dmap (fin sfuncs) (fun f => list (hlist (expr fs vars) (SDomain (get sfuncs f))))
-       -> map (expr fs vars pcType) (sexpr fs sfuncs consts (stateType :: vars))
+       -> fmap (expr fs vars pcType) (sexpr fs sfuncs consts (stateType :: vars))
        -> list (expr fs vars None)
        -> list (fin consts)
        -> list (sexpr fs sfuncs consts vars) -> T) : T :=
-      @hash_rec T vars s cc dmap_empty (map_empty _ _) nil nil nil.
+      @hash_rec T vars s cc dmap_empty fmap_empty nil nil nil.
 
     Section WithCS.
     Variable cs : codeSpec (tvarD pcType) (tvarD stateType).
-
-(*
-    Existing Instance M.Refl_himp.
-    Existing Instance M.Trans_himp.
-*)
 
     Ltac cancel_all :=
       repeat apply star_assoc_p;
         do 10 (repeat eapply star_assoc_c;
           (reflexivity || simple apply star_emp_c || simple apply star_emp_p || simple apply star_cancel || simple apply star_comm_c)).
+
+    Lemma fold_star : forall K V vars G (ctor : forall k : K, V k -> sexpr fs sfuncs consts vars) (B : @dmap K V) P Q,
+      himp stateMem G cs
+        (Star Q (dmap_fold (fun (a : sexpr fs sfuncs consts vars) (k : K) (v : V k) => Star (ctor k v) a) P B))
+        (Star P
+          (dmap_fold (fun (a : sexpr fs sfuncs consts vars) (k : K) (v : V k) => Star (ctor k v) a) Q B)
+        ).
+    Proof.
+      induction B; simpl; intros. cancel_all. etransitivity. eapply IHB2. etransitivity. 2: eapply IHB2.
+      etransitivity. eapply star_frame. etransitivity; [ | apply (IHB1 (Star (ctor k v) P) Emp) ]; cancel_all.
+      etransitivity; [ | apply (IHB2 Q Emp) ]; cancel_all.
+      etransitivity. Focus 2.
+      eapply star_frame. etransitivity; [ eapply (IHB1 Emp (Star (ctor k v) Q)) | ]; cancel_all.
+      etransitivity; [ eapply (IHB2 Emp P) | ]; cancel_all. cancel_all.
+    Qed.
+
+    Lemma fold_star' : forall K V vars G (ctor : forall k : K, V k -> sexpr fs sfuncs consts vars) (B : @dmap K V) P,
+      himp stateMem G cs
+        (dmap_fold (fun (a : sexpr fs sfuncs consts vars) (k : K) (v : V k) => Star (ctor k v) a) P B)
+        (Star P
+          (dmap_fold (fun (a : sexpr fs sfuncs consts vars) (k : K) (v : V k) => Star (ctor k v) a) Emp B)
+        ).
+    Proof.
+      intros. etransitivity; [ | eapply fold_star ]. cancel_all.
+    Qed.
+
+    Lemma fold_star'' : forall K V vars G (ctor : forall k : K, V k -> sexpr fs sfuncs consts vars) (B : @dmap K V) P,
+      himp stateMem G cs
+        (Star P
+          (dmap_fold (fun (a : sexpr fs sfuncs consts vars) (k : K) (v : V k) => Star (ctor k v) a) Emp B))
+        (dmap_fold (fun (a : sexpr fs sfuncs consts vars) (k : K) (v : V k) => Star (ctor k v) a) P B).
+    Proof.
+      intros. etransitivity; [ eapply fold_star | ]. cancel_all.
+    Qed.
+
+(*
+    Lemma fold_fold : forall K V vars G (ctor : forall k : K, V k -> sexpr fs sfuncs consts vars) (cmp : forall a b : K, option (dcomp a b)) (B B' : @dmap K V) P,
+      himp stateMem G cs
+        (dmap_fold (fun (a : sexpr fs sfuncs consts vars) (k : K) (v : V k) => Star (ctor k v) a) 
+          (dmap_fold (fun (a : sexpr fs sfuncs consts vars) (k : K) (v : V k) => Star (ctor k v) a) P B) B')
+        (Star
+          (dmap_fold (fun (a : sexpr fs sfuncs consts vars) (k : K) (v : V k) => Star (ctor k v) a) Emp B) 
+          (dmap_fold (fun (a : sexpr fs sfuncs consts vars) (k : K) (v : V k) => Star (ctor k v) a) P B')
+        ).
+    Proof.
+      induction B; simpl; intros. cancel_all.
+      etransitivity. eapply IHB2. etransitivity. instantiate (1 := Star (dmap_fold
+           (fun (a : sexpr fs sfuncs consts vars) (k0 : K) (v0 : V k0) =>
+            Star (ctor k0 v0) a) Emp B2) (Star (dmap_fold
+         (fun (a : sexpr fs sfuncs consts vars) (k0 : K) (v0 : V k0) =>
+          Star (ctor k0 v0) a) P B') (dmap_fold
+            (fun (a : sexpr fs sfuncs consts vars) (k0 : K) (v0 : V k0) =>
+             Star (ctor k0 v0) a) (Star (ctor k v) Emp) B1))). cancel_all. etransitivity. eapply IHB1.
+*)
+
+    Lemma star_insert : forall K V vars G (ctor : forall k : K, V k -> sexpr fs sfuncs consts vars) (cmp : forall a b : K, option (dcomp a b)) (B : @dmap K V) k (v : V k) P,
+      himp stateMem G cs
+        (dmap_fold
+          (fun (a : sexpr fs sfuncs consts vars) (k : K) (v : V k) =>
+            Star (ctor k v) a) P (@dmap_insert _ _ cmp k v B))
+        (Star
+          (dmap_fold
+            (fun (a : sexpr fs sfuncs consts vars) (k : K) (v : V k) => Star (ctor k v) a) P B) (ctor k v)).
+    Proof.      
+      clear. induction B. simpl. intros. apply star_comm_p. reflexivity.
+      simpl. intros. destruct (cmp k k0). destruct d; simpl in *. etransitivity; [ eapply fold_star' | ].
+      apply star_comm_c. etransitivity; [ | eapply fold_star ].
+    Admitted.
 
     Lemma denote_hash_rec : forall vars (s : sexpr fs sfuncs consts vars) P (cc : _ -> _ -> _ -> _ -> _ -> SHeap vars) G,
       (forall A B C D E, 
@@ -482,7 +558,29 @@ Module SepExpr (B : Heap).
         (* Star *)
         etransitivity. eapply IHs1. intros. etransitivity. eapply IHs2. intros. etransitivity. eapply H. reflexivity.
         instantiate (1 := Star P s2). cancel_all. repeat cancel_all.
+        (* Cptr *) Focus.
+        etransitivity. eapply H. unfold denote; simpl. cancel_all. apply star_comm_p. cancel_all. cancel_all.
+        clear.
+        match goal with
+          | [ |- context [ @Emp ?A ?B ?C ?D ?E ?F ?G ] ] => generalize (@Emp A B C D E F G)
+        end. induction B; intros; simpl. apply star_comm_p. reflexivity. etransitivity. unfold fmap_fold. eapply fold_star'.
+        etransitivity. eapply star_frame. eapply IHB1. reflexivity. cancel_all. etransitivity. eapply star_frame.
+        unfold fmap_fold. eapply fold_star'. reflexivity. cancel_all. etransitivity. 2: eapply star_frame.
+        2: unfold fmap_fold; eapply fold_star''. 2: reflexivity. apply star_assoc_c. etransitivity.
+        2: eapply star_frame. 2: eapply fold_star''. 2: reflexivity. cancel_all.
+        (** Func **) Focus.
     Admitted.
+
+    Lemma denote_hash_rec' : forall vars (s : sexpr fs sfuncs consts vars) P (cc : _ -> _ -> _ -> _ -> _ -> SHeap vars) G,
+      (forall A B C D E, 
+        himp stateMem G cs 
+          (Star P (denote (Build_SHeap D E A B C)))
+          (denote (cc D E A B C))) ->
+      forall A B C D E,
+      himp stateMem G cs (Star (Star (denote (Build_SHeap A B C D E)) P) s) (denote (hash_rec s cc A B C D E)).
+    Proof.
+    Admitted.
+
 
     Theorem denote_hash_cc : forall (s : sexpr fs sfuncs consts nil),
       Himp stateMem cs (denote (hash_cc s (@Build_SHeap nil))) s.
@@ -490,13 +588,14 @@ Module SepExpr (B : Heap).
       unfold Himp. intros. unfold hash_cc. etransitivity. eapply denote_hash_rec.
       instantiate (1 := Emp). intros. 
       generalize (denote {| funcs := D; cptrs := E; pures := A; cnsts := B; other := C |}).
-      intros; cancel_all. unfold denote. simpl. rewrite map_fold_empty. 
+      intros; cancel_all. unfold denote. simpl. 
       repeat (apply star_emp_p || apply star_assoc_p). reflexivity.
     Qed.
 
     Theorem denote_hash_cc_p : forall (s : sexpr fs sfuncs consts nil),
       Himp stateMem cs s (denote (hash_cc s (@Build_SHeap nil))).
     Proof.
+      unfold Himp. intros. unfold hash_cc. etransitivity. 
     Admitted.
 
 
@@ -556,7 +655,7 @@ Module SepExpr (B : Heap).
         with
         | Emp _ => fun h rem => (h, rem)
         | Func _ f a => fun h rem =>
-          match dmap_remove (@finCmp _ _) f (funcs h) with
+          match dmap_remove (fun x y => Some (@finCmp _ _ x y)) f (funcs h) with
             | Some (ls, fs') => 
               match take_out (fun x y => if hlistEq (@exprEq _ _ _ ) x y then true else false) a ls nil with
                 | None => (h,rem)
@@ -568,7 +667,7 @@ Module SepExpr (B : Heap).
                     ; cnsts := cnsts h
                     |}, rem)
                 | Some v =>
-                  ({| funcs := dmap_insert (@finCmp _ _) f v fs'
+                  ({| funcs := dmap_insert (fun x y => Some (@finCmp _ _ x y)) f v fs'
                     ; cptrs := cptrs h
                     ; pures := pures h
                     ; other := other h
@@ -578,10 +677,10 @@ Module SepExpr (B : Heap).
             | None => (h,rem)
           end              
         | Cptr _ p s => fun h rem =>
-          match map_remove p (cptrs h) with
+          match fmap_remove (@exprCmp _ _ _ _) p (cptrs h) with
             | Some (s', cp') => 
               match sexprCmp s s' with
-                | Env.Eq _ => 
+                | Some (Env.Eq _) => 
                 ({| funcs := funcs h 
                   ; cptrs := cp'
                   ; pures := pures h
@@ -627,7 +726,7 @@ Module SepExpr (B : Heap).
     Proof.
       unfold Himp; intros. etransitivity. eapply sepCancel_cancels'. eassumption.
       instantiate (1 := Emp). etransitivity. eassumption. generalize (denote rr).
-      intros; cancel_all. unfold denote. simpl. rewrite map_fold_empty. 
+      intros; cancel_all. unfold denote. simpl. 
       repeat (apply star_comm_p; repeat apply star_assoc_p; apply star_emp_p).
       apply star_comm_p;
         repeat (apply star_comm_p; repeat apply star_assoc_p; apply star_emp_p).
@@ -654,16 +753,62 @@ Module SepExpr (B : Heap).
       unfold lhs. etransitivity. eapply denote_hash_cc_p. reflexivity.
     Defined.
 
-
   End BabySep.
 
+  (** Tests **)
+  Section ProverTests.
+    Require Import Arith.
+    Variable pcType : Type.
+    Variable stateType : Type.
+
+    Definition types := 
+      {| Impl := pcType ; Eq := fun _ _ => None |} ::
+      {| Impl := stateType ; Eq := fun _ _ => None |} ::
+      {| Impl := nat; Eq := fun x y => match eq_nat_dec x y with left Heq => Some Heq | _ => None end |} :: nil.
+
+    Definition fs : functions types :=
+       {| Domain := Some (FS (FS FO)) :: Some (FS (FS FO)) :: nil;
+          Range := None; Denotation := eq |}
+    :: {| Domain := (Some (FS (FS FO)) :: Some (FS (FS FO)) :: nil) : list (tvar types);
+          Range := Some (FS (FS FO)); Denotation := plus |}
+    :: nil.
+
+    Definition pcTypeV : tvar types := Some FO.
+    Definition stateTypeV : tvar types := Some (FS FO).
+
+    Definition consts : list (PropX (tvarD pcTypeV) (tvarD stateTypeV)) := nil.
+    Definition vars : variables types := nil.
+
+    Parameter repr : nat -> hprop pcTypeV stateTypeV.
+
+    Variable stateMem : tvarD stateTypeV -> B.mem.
+    Definition sfuncs : list (@ssignature types pcTypeV stateTypeV) :=
+      {| SDomain := Some (FS (FS FO)) :: nil
+       ; SDenotation := repr
+         : functionTypeD (map (@tvarD types) (Some (FS (FS FO)) :: nil)) (hprop pcTypeV stateTypeV)
+       |} :: nil.
+    
+About Func.
+  Goal forall cs,
+    Himp stateMem cs (@Func types fs pcTypeV stateTypeV sfuncs consts vars FO (HCons (Expr.Const fs vars (Some (FS (FS FO))) 1) HNil))
+                     (@Func types fs pcTypeV stateTypeV sfuncs consts vars FO (HCons (Expr.Const fs vars (Some (FS (FS FO))) 1) HNil)).
+  Proof.
+    intros.
+    match goal with
+      | [ |- Himp ?M ?C ?L ?R ] =>
+        let R := fresh in
+        let rr := eval hnf in (@CancelSep types fs pcTypeV stateTypeV M sfuncs consts C nil L R) in
+        match rr with
+          | Proved ?PF => exact PF
+          | Remaining _ _ ?PF => apply PF; unfold denote; simpl
+        end
+    end. reflexivity.
+    Defined.
   
-
-
   Section QSexpr.
     (** Guarded separation logic expressions **)
   End QSexpr.
-    
 
 End SepExpr.
+
 Require Export Expr.
