src/Reflect.v
@@ -1,0 +1,59 @@
+(** Reusable Ltac procedures:
+ ** - reflecting function applications
+ ** - list lookup
+ ** - 
+ **)
+Require Import List Env.
+
+Set Implicit Arguments.
+
+Section PartialApply.
+  Fixpoint funtype (ls : list Type) (r : Type) : Type :=
+    match ls with 
+      | nil => r
+      | a :: b => a -> funtype b r
+    end.
+
+  Fixpoint apply_ls (ls : list Type) (T : Type) (R : T -> Type) (V : T)
+    : funtype ls (forall x : T, R x) -> funtype ls (R V) :=
+    match ls with
+      | nil => fun F => F V
+      | a :: b => fun F => fun x : a => apply_ls b R V (F x)
+    end.
+End PartialApply.
+
+(** Reflect an application
+ ** - reflects all the non-dependent arguments of e into a tuple
+ ** - the tuple and the resulting function (may be partially applied)
+ **   are passed to the continuation [cc]
+ **) 
+Ltac refl_app cc e := 
+  let rec refl cc e As :=
+    match e with
+      | ?A ?B =>
+        let Ta := type of A in
+        match type of A with
+          | _ -> ?TT => 
+            let As := constr:((B, As)) in
+            let Tb := type of B in
+            let cc f Ts args := 
+              let Ts' := constr:(Ts ++ (Tb : Type) :: nil) in
+              cc f Ts' args
+            in 
+            refl cc A As
+          | forall x : ?T1, @?T2 x => 
+            let cc f Ts args := 
+              let Tb  := type of B in
+              let f'  := eval simpl in (@apply_ls Ts T1 T2 B f) in
+              cc f' Ts args
+            in
+            refl cc A As
+        end
+      | _ =>
+        let Ts := constr:(@nil Type) in
+        cc e Ts As
+    end
+  in
+  let b := constr:(tt) in
+  refl cc e b.
+
